App/Lib/NatRangeIterator/Props.v
@@ -13,20 +13,20 @@ Ltac destruct_wf_ex H var ref at_start count Hvar Hsk Hsr :=
 Section Props.
 Open Scope oo_scope.
 
-Variable step : step_relation.
+Variable exec_step : exec_step_relation.
 
-Notation "t1 '/' st1 '==>' t2 '/' st2" := (step (Cexec_state t1 st1) (Cexec_state t2 st2))
+Notation "t1 '/' st1 '==>' t2 '/' st2" := (exec_step (Cexec_state t1 st1) (Cexec_state t2 st2))
   (at level 40, st1 at level 39, t2 at level 39, format "'[' t1 / st1 '==>' t2 / st2 ']'").
 
-Notation "t1 '/' st1 '==>*' t2 '/' st2" := (multi step (Cexec_state t1 st1) (Cexec_state t2 st2))
+Notation "t1 '/' st1 '==>*' t2 '/' st2" := (multi exec_step (Cexec_state t1 st1) (Cexec_state t2 st2))
   (at level 40, st1 at level 39, t2 at level 39, format "'[' t1 / st1 '==>*' t2 / st2 ']'").
 
-Variable proof_get_at_start : get_at_start step.
+Variable proof_get_at_start : get_at_start exec_step.
 
 Definition terminates_get_at_start:
   forall x st,
   wf_ex x st ->
-  term_terminates step (x # "get_at_start"|()|) st.
+  term_terminates exec_step (x # "get_at_start"|()|) st.
 Proof.
   intros.
   destruct_wf_ex H var ref at_start count Hvar Hsk Hsr.
@@ -47,24 +47,24 @@ Module IteratorVerification.
 Section ConformsToIterator.
 Open Scope oo_scope.
 
-Variable step : step_relation.
+Variable exec_step : exec_step_relation.
 
-Notation "t1 '/' st1 '==>' t2 '/' st2" := (step (Cexec_state t1 st1) (Cexec_state t2 st2))
+Notation "t1 '/' st1 '==>' t2 '/' st2" := (exec_step (Cexec_state t1 st1) (Cexec_state t2 st2))
   (at level 40, st1 at level 39, t2 at level 39, format "'[' t1  /  st1  '==>'  t2  /  st2 ']'").
 
-Notation "t1 '/' st1 '==>*' t2 '/' st2" := (multi step (Cexec_state t1 st1) (Cexec_state t2 st2))
+Notation "t1 '/' st1 '==>*' t2 '/' st2" := (multi exec_step (Cexec_state t1 st1) (Cexec_state t2 st2))
   (at level 40, st1 at level 39, t2 at level 39, format "'[' t1  /  st1  '==>*'  t2  /  st2 ']'").
 
-Variable proof_off_true : off_true step.
-Variable proof_off_false : off_false step.
-Variable proof_after_true : after_true step.
-Variable proof_after_false : after_false step.
-Variable proof_forth_at_start : forth_at_start step.
-Variable proof_forth : forth step.
-Variable proof_item : item step.
+Variable proof_off_true : off_true exec_step.
+Variable proof_off_false : off_false exec_step.
+Variable proof_after_true : after_true exec_step.
+Variable proof_after_false : after_false exec_step.
+Variable proof_forth_at_start : forth_at_start exec_step.
+Variable proof_forth : forth exec_step.
+Variable proof_item : item exec_step.
 
 Theorem deterministic_off:
-  Iterator.Spec.deterministic_off step wf_ex.
+  Iterator.Spec.deterministic_off exec_step wf_ex.
 Proof.
   unfold deterministic_off. intros.
   destruct_wf_ex H var ref at_start count Hvar Hsk Hsr.
@@ -79,32 +79,32 @@ Proof.
   Abort.
 
 Theorem terminates_off:
-  Iterator.Spec.terminates_off step wf_ex.
+  Iterator.Spec.terminates_off exec_step wf_ex.
 Proof.
   Abort.
 
 Theorem preserves_wf_off:
-  Iterator.Spec.preserves_wf_off step wf_ex.
+  Iterator.Spec.preserves_wf_off exec_step wf_ex.
 Proof.
   Abort.
 
 Theorem returns_tbool_off:
-  Iterator.Spec.returns_tbool_off step wf_ex.
+  Iterator.Spec.returns_tbool_off exec_step wf_ex.
 Proof.
   Abort.
 
 Theorem perserves_off_off:
-  Iterator.Spec.perserves_off_off step wf_ex.
+  Iterator.Spec.perserves_off_off exec_step wf_ex.
 Proof.
   Abort.
 
 Theorem perserves_off_after:
-  Iterator.Spec.perserves_off_after step wf_ex.
+  Iterator.Spec.perserves_off_after exec_step wf_ex.
 Proof.
   Abort.
 
 Theorem perserves_off_item:
-  Iterator.Spec.perserves_off_item step wf_ex.
+  Iterator.Spec.perserves_off_item exec_step wf_ex.
 Proof.
   Abort.
 
