App/Lib/NatRangeIterator/Step.v
@@ -10,7 +10,7 @@ Open Scope oo_scope.
 Reserved Notation "t1 '/' st1 '==>' t2 '/' st2"
   (at level 40, st1 at level 39, t2 at level 39).
 
-Inductive step : step_relation :=
+Inductive exec_step : exec_step_relation :=
   | STexec_NatRangeIterator_make :
     forall st,
     texec "NatRangeIterator_make" / st ==> (
@@ -114,18 +114,18 @@ Inductive step : step_relation :=
       this#"get_first"|()|
     )) / resize_sk_hd 1 st
 
-  where "t1 '/' st1 '==>' t2 '/' st2" := (step (Cexec_state t1 st1) (Cexec_state t2 st2)).
+  where "t1 '/' st1 '==>' t2 '/' st2" := (exec_step (Cexec_state t1 st1) (Cexec_state t2 st2)).
 
-Lemma value_irreducible__step:
-  value_irreducible step.
+Lemma value_irreducible__exec_step:
+  value_irreducible exec_step.
 Proof with auto.
   intros t Hval.
   induction Hval;
   try solve [intros t' st st' Hcontra; inversion Hcontra].
   Qed.
 
-Lemma deterministic__step:
-  deterministic step.
+Lemma deterministic__exec_step:
+  deterministic exec_step.
 Proof with auto.
   intros x y Hxy.
   induction Hxy; intros z Hxz; inversion Hxz; subst;
