App/Feasibility.v
@@ -9,13 +9,13 @@ Require Import App.Lib.NatRangeIterator.Props.
 Import ObjectOrientedNotations.
 Import StateNotations.
 
-Notation "t1 '/' st1 '==>' t2 '/' st2" := (step (Cexec_state t1 st1) (Cexec_state t2 st2))
+Notation "t1 '/' st1 '==>' t2 '/' st2" := (exec_step (Cexec_state t1 st1) (Cexec_state t2 st2))
   (at level 40, st1 at level 39, t2 at level 39, format "'//' '[' t1 '//' / '//' st1 '//' '==>' '//' t2 '//' / '//' st2 ']'").
 
-Notation "t1 '/' st1 '==>*' t2 '/' st2" := (multi step (Cexec_state t1 st1) (Cexec_state t2 st2))
+Notation "t1 '/' st1 '==>*' t2 '/' st2" := (multi exec_step (Cexec_state t1 st1) (Cexec_state t2 st2))
   (at level 40, st1 at level 39, t2 at level 39, format "'['  t1  /  st1  '==>*'  t2  /  st2 ']'").
 
-Ltac reduce_step := Language.reduce_step || NatRangeIterator.reduce_step.
+Ltac reduce_exec_step := Language.reduce_exec_step || NatRangeIterator.reduce_exec_step.
 
 Ltac rewrite_nth :=
   match goal with
@@ -24,10 +24,10 @@ Ltac rewrite_nth :=
 
 Ltac reduce :=
   match goal with
-  | |- multi step _ _ => solve [apply Relation_Operators.rt1n_refl]
-  | |- multi step _ _ => 
+  | |- multi exec_step _ _ => solve [apply Relation_Operators.rt1n_refl]
+  | |- multi exec_step _ _ => 
     eapply Relation_Operators.rt1n_trans;
-    [repeat reduce_step | instantiate; simpl; repeat rewrite_nth; fold multi]
+    [repeat reduce_exec_step | instantiate; simpl; repeat rewrite_nth; fold multi]
   end.
 
 Open Scope oo_scope.
@@ -53,7 +53,7 @@ Ltac expand_wf_ex :=
   end.
 
 Theorem off__no_side_effects:
-  Iterator.Spec.off__no_side_effects step NatRangeIterator.Spec.wf_ex.
+  Iterator.Spec.off__no_side_effects exec_step NatRangeIterator.Spec.wf_ex.
 Proof.
   unfold off__no_side_effects.
   intros. expand_wf_ex. subst x.
@@ -68,7 +68,7 @@ Proof.
   Abort.
 
 Theorem proof_get_at_start:
-  Spec.get_at_start step.
+  Spec.get_at_start exec_step.
 Proof.
   unfold get_at_start.
   unfold wf. intros.
@@ -83,8 +83,8 @@ Proof.
 Theorem terminates_get_at_start :
   forall x st,
   wf_ex x st ->
-  term_terminates step (x # "get_at_start"|()|) st.
+  term_terminates exec_step (x # "get_at_start"|()|) st.
 Proof.
-  apply (terminates_get_at_start step proof_get_at_start).
+  apply (terminates_get_at_start exec_step proof_get_at_start).
   Qed.
 
